src/cbor/pulse/raw/everparse/CBOR.Pulse.Raw.EverParse.Nondet.Basic.fst
@@ -68,6 +68,29 @@ let impl_check_equiv_basic
 : impl_equiv_t #_ (check_equiv basic_data_model (option_sz_v map_bound))
 = impl_check_equiv map_bound (impl_check_equiv_list_basic map_bound)
 
+fn impl_list_for_all_with_overflow_setoid_assoc_eq_with_overflow_basic
+  (nl1: SZ.t)
+  (l1: S.slice byte)
+  (nl2: SZ.t)
+  (l2: S.slice byte)
+  (#pl1: perm)
+  (#gl1: Ghost.erased (nlist (SZ.v nl1) (raw_data_item & raw_data_item)))
+  (#pl2: perm)
+  (#gl2: Ghost.erased (nlist (SZ.v nl2) (raw_data_item & raw_data_item)))
+requires
+  pts_to_serialized (serialize_nlist (SZ.v nl1) (serialize_nondep_then serialize_raw_data_item serialize_raw_data_item)) l1 #pl1 gl1 **
+  pts_to_serialized (serialize_nlist (SZ.v nl2) (serialize_nondep_then serialize_raw_data_item serialize_raw_data_item)) l2 #pl2 gl2
+returns res: option bool
+ensures
+  pts_to_serialized (serialize_nlist (SZ.v nl1) (serialize_nondep_then serialize_raw_data_item serialize_raw_data_item)) l1 #pl1 gl1 **
+  pts_to_serialized (serialize_nlist (SZ.v nl2) (serialize_nondep_then serialize_raw_data_item serialize_raw_data_item)) l2 #pl2 gl2 **
+  pure (
+    res == list_for_all_with_overflow (setoid_assoc_eq_with_overflow (check_equiv basic_data_model None) (check_equiv basic_data_model None) gl1) gl2
+  )
+{
+  impl_list_for_all_with_overflow_setoid_assoc_eq_with_overflow (impl_check_equiv_basic None) nl1 l1 nl2 l2
+}
+
 let impl_check_valid_basic
   (map_bound: option SZ.t)
   (strict_bound_check: bool)
